# Algebraic Expression

1. Write the following using literals, numbers and signs of basic operations.
   (a) x increased by 12
   (b) y decreased by 7
   (c) The difference of a and b. when a > b
   (d) 5 times x added to 7 times y
   (e) Sum of x and the quotient of y by 5
   (f) x taken away from 4
   (g) 2 less than the quotient of x by y
   (h) x multiplied by itself
   (i) Twice x increased by y
   (j) Thrice x added to y squared
   (k) x cubed less than y cubed
2. Write the following in the exponential form:
   (a) b × b × b × …15 times
   (b) y × y × y × …20 times
   (c) 14 × a × a × a × a × b × b × b
   (d) 6 × x × x × y × y
   (e) 3 × z × z × z × y × y × x
3. Write down the following in the product form:
   (a) x^2^y^4^
   (b) 6y^5^
   (c) 9xy^2^z
   (d) 10a^3^b^3^c^3^
4. If a = 2 and b = 3. find the value of
   (a) a + b
   (b) a^2^ + ab
   (c) ab − a^2^
   (d) 2a − 3b
   (e) 5a^2^ − 2ab
   (f) a^3^ − b^3^
5. If x = 1, y = 2 and z = 5, find the value of
   (a) 3x − 2y + 4z
   (b) x^2^ + y^2^ + z^2^
   (c) 2x^2^ − 3y^2^ + z^2^
   (d) xy + yz − zx
   (e) 2x^2^y − 5yz + xy^2^
   (f) x^3^ − y^3^ − z^3^
6. If p = −2, q = −1 and r = 3, find the value of
   (a) p^2^ + q^2^ − r^2^
   (b) 2p^2^ − q^2^ + 3r
   (c) p − q − r
   (d) p^3^ + q^3^ + r^3^ + 3pqr
   (e) p^4^ +q^4^ - r^4^
   (f) 3p^2^q + 5pq^2^ + 2pqr
7. Write the coefficient of
   (a) x in 13x
   (b) y in −5y
   (c) y^2^ in 8xy^2^z
   (d) z in −7xz
   (e) p in −2pqr
   (f) a in 6ab
   (g) x^3^ in x^3^
   (i) x^2^ in −x^2^
   (j) x^2^ in &pi;x^2^
8. Write the numerical coefficient of
   (a) ab
   (b) −6bc
   (c) 7xyz
   (d) −2x^3^y^2^z
   (e) −bc^2^
9. Write the constant term of
   (a) 3x^2^ + 5x + 8
   (b) 2x^2^ − 9
   (c) 4y^2^ − 5y + $\frac{3}{5}$
   (d) z^3^ - 2z^2^ + z − $\frac{8}{3}$
10. Identify the monomials, binomials and trinomials in the following:
    (a) −2xyz
    (b) 5 + 7x^3^y^3^z^3^
    (c) −5x^3^
    (d) a + b − 2c
    (e) xy + yz - zx
    (f) x^5^
    (g) 2x + 1
    (i) −14
    (j) ax^3^ + bx^3^ + cx + d
11. Write all the terms of the algebraic expressions:
    (a) 4x^5^ − 6y^4^ + 7x^2^y − 9
    (b) 9x^3^ − 5z^4^ + 7x^3^y − xyz
12. Identify the like terms in the following:
    (a) a^2^, b^2^, −2a^2^, c^2^ , 4a
    (b) 3x, 4xy, −yz, −zy, $\frac{1}{2}$zy
    (c) −2xy^2^, x^2^y, 5y^2^x, x^2^z
    (d) abc, ab^2^c, acb^2^, c^2^ab, b^2^ac, a^2^bc, cab^2^

**Add:**

13. (a) 3x, 7x
    (b) 7y, −9y
    (c) 2xy 5xy, −xy
    (d) 3x, 2y
    (e) 2x^2^, 3x^2^, 7x^2^
    (f) 6a^3^, −4a^3^, 10a^3^, − 8a^3^
    (g) 7xyz, −5xyz, 9xyz, − 8xyz
    (i) x^2^ −a^2^, − 5x^2^ + 2a^2^, − 4x^2^ + 4a^2^
14. (a) x − 3y − 2z, 5x + 7y − z and −7x − 2y + 4z
    (b) m^2^ − 4m + 5, −2m^2^ + 6m − 6 and −m^2^ − 2m − 7
    (c) 2x^2^ − 3xy + y^2^, −7x^2^ − 5xy − 2y^2^ and 4x^2^ + xy − 6y^2^
    (d) 4xy − 5yz − 7zx, −5xy + 2yz + zx and −2xy − 3yz + 3zx
15. (a) 3a − 2b + 5c, 2a + 5b − 7c, − a − b + c
    (b) 8a − 6ab + 5b, 6a − ab − 8b, − 4a + 2ab + 3b
    (c) 2x^3^ − 3x^2^ + 7x − 8, − 5x^3^ + 2x^2^ − 4x + 1, 3 − 6x + 5x^2^ − x^3^
    (d) 2x^2^ − 8xy + 7y^2^ − 8xy^2^, 2xy^2^ + 6xy − y^2^ + 3x^2^, 4y^2^ − xy − x^2^ + xy^2^
    (e) x^3^ + y^3^ − Z^3^ + 3xyz, − x^3^ + y^3^ + z^3^ − 6xyz, x^3^ − y^3^ − z
    (f) 2 + x − x^2^ + 6x^3^, − 6 − 2x + 4x^2^ − 3x^3^, 2 + x^2^, 3 − x^3^ + 4x − 2x

**Subtract:**

14. (a) 5x from 2x
    (b) −xy from 6xy
    (c) 3a from 5b
    (d) −7x from 9y
    (e) 10x^2^ from −7x^2^
    (f) a^2^ − b^2^ from b^2^ − a^2^
15. (a) 5a + 7b − 2c from 3a − 7b + 4c
    (b) a − 2b − 3c from −2a + 5b − 4c
    (c) 5x^2^ − 3xy + y^2^ from 7x^2^ − 2xy − 4y^2^
    (d) 6x^3^ − 7x^2^ + 5x − 3 from 4 − 5x + 6x^2^ − 8x^3^
    (e) x^3^ + 2x^2^y + 6xy^2^ − y^3^ from y^3^ − 3xy^2^
    (f) −11x^2^y^2^ + 7xy − 6 from 9x^2^y^2^ − 6xy + 9
    (g) −2a + b + 6d from 5a − 2b − 3c

**Simplify:**

15. (a) 2p^3^ − 3p^2^ + 4p^5^ − 6p^3^ + 2p^2^ − 8p − 2 + 6p + 8
    (b) 2x^2^ − xy + 6x − 4y + 5xy − 4x + 6x + 3y
    (c) x^4^ − 6x^3^ + 2x − 7 + 7x^3^ − x + 5x^2^ + 2 − x^4^
16. (a) a − (b − 2a)
    (b) 4x − (3y − x + 2z)
17. (a) (a^2^ + b^2^ + 2ab) − (a^2^ + b^2^ − 2ab)
    (b) −3(a + b) + 4(2a − 3b) − (2a − b)
    (c) −4x^2^ + {(2x^2^ − 3) − (4 − 3x^2^)}
    (d) −2(x^2^ − y^2^ + xy) − 3(x^2^ + y^2^ − xy)
    (e) a − [2b − {3a − (2b − 3c)}]
    (f) − x + [5y − {x − (5y − 2x)}]
    (g) 86 − [15x − 7(6x − 9) − 2{10x − 5(2 − 3x)}]
    (h) 12x − [3x^2^ + 5x^2^ − {7x^2^ − (4 − 3x − x^3^) + 6x^3^} − 3x]
    (i) 5a − [a^2^ − {2a(1 − a + 4a^2^)− 3a(a^2^ − 5a^3^)}] − 8a
    (j) 3 − [x − {2y −(5x + y − 3) + 2x^2^} −(x^2^ − 3y)]
    (k) xy − [yz − zx − {yx −(3y − xz)−(xy − zy)}]
    (l) 2a − 3b − [3a − 2b − {a − c − (a − 2b)}]
    (m) −a − [a + {a + b − 2a − (a − 2b)} − b]

# Simple Equations

1. Write each of the following statements as an equation:
   (a) 5 times a number equals 40.
   (b) A number Increased by 8 equals 15.
   (c) 25 exceeds a number by 7.
2. Write a statement for each of the equations, given below:
   (a) x − 7 = 14
   (b) 2y = 18
   (c) 11 + 3x = 17
   (d) 2x − 3 = 13
   (e) 12y − 30 = 6
   (f) $\frac{2z}{3}$ = 8
3. Verify by substitution that
   (a) the root of 3x − 5 = 7 is x = 4
   (b) the root of 3 + 2x = 9 is x = 3
4. Solve each of the following equations by the trial-and-error method:
   (a) y + 9 = 13
   (b) x − 7 = 10
   (c) 4x = 28
   (d) 3y = 36
   (e) 11 + x = 19
   (f) $\frac{x}{3}$ = 4

Solve each, of the following equations and. verify the answer in each case:

1. (a) x – 1 = 0
   (b) x + 1 = 0
   (c) x – 1 = 5
   (d) x + 6 = 2
   (e) y – 4 = –7
   (f) y – 4 = 4
   (g) y + 4 = 4
   (h) y + 4 = –4
2. (a) 3l = 42
   (b) $\frac{b}{2}$ = 6
   (c) $\frac{p}{7}$ = 4
   (d) 4x = 25
   (e) 8y = 36
   (f) $\frac{z}{3}$ = $\frac{5}{4}$
   (g) $\frac{a}{5}$ = $\frac{7}{15}$
   (h) 20t = –10
3. (a) 3n – 2 = 46
   (b) 5m + 7 = 17
   (c) $\frac{20p}{3}$ = 40
   (d) $\frac{3p}{10}$ = 6
4. (a) 10p = 100
   (b) 10p + 10 = 100
   (c) $\frac{\text{p}}{4} = 5$
   (d) $\frac{\text{–P}}{3} = 5$
   (e) $\frac{3p}{4} = 6$
   (f) 3s = –9
   (g) 3s + 12 = 0
   (h) 3s = 0
   (i) 2q = 6
   (k) 2q – 6 = 0
   (k) 2q + 6 = 0
   (l) 2q + 6 = 12
5. (a) 2y + $\frac{5}{2}$ = $\frac{37}{2}$
   (b) 5t + 28 = 10
   (c) $\frac{a}{5}$ + 3 = 2
   (d) $\frac{q}{4}$ + 7 = 5
   (e) $\frac{5}{2}$x = 10
   (f) $\frac{5}{2}$x = $\frac{52}{4}$
   (g) 7m + $\frac{19}{2}$ = 13
   (h) 6z + 10 = –2
   (i) $\frac{3l}{2}$ = $\frac{2}{3}$
   (k) $\frac{2b}{3}$ – 5 = 3
6. (a) 2(x + 4) = 12
   (b) 3(n – 5) = 21
   (c) 3(n – 5) = – 21
   (d) – 4(2 + x) = 8
   (e) 4(2 – x) = 8
7. (a) 4 = 5(p – 2)
   (b) – 4 = 5(p – 2)
   (c) 16 = 4 + 3(t + 2)
   (d) 4 + 5(p – 1) = 34
   (e) 0 = 16 + 4(m – 6)

# Exponents and Powers

1. Find the value of:
   (a) 2^6^
   (b) 9^3^
   (c) 11^2^
   (d) 5^4^
   (e) 6^7^
   (f) 12^3^
2. Express the following in exponential form:
   (a) 6 × 6 × 6 × 6
   (b) t × t
   (c) b × b × b × b
   (d) 5 × 5 × 7 × 7 × 7
   (e) 2 × 2 × a × a
   (f) a × a × a × c × c × c × c × d
3. Express each of the following numbers using exponential notation:
   (a) 512
   (b) 343
   (c) 729
   (d) 3125
   (e) 625
4. Identify the greater number, wherever possible, in each of the following?
   (a) 4^3^ या 3^4^
   (b) 5^3 या 3^5^
   (c) 2^8^ या 8^2^
   (d) 2^3^ या 2^2^
5. Express each of the following as product of powers of their prime factors:
   (a) 648
   (b) 405
   (c) 540
   (d) 3600
   (e) 7200

**Simplify:**

6. (a) 2 × 10^3^
   (b) 72 × 2^2^
   (c) 2^3^ × 5
   (d) 3 × 4^4^
   (e) 0 × 10^2^
   (f) 5^2^ × 3^3^
   (g) 2^4^ × 3^2^
   (h) 3^2^ × 10^4^
7. Simplify:
   (a) (–4)^3^
   (b) (–3) × (–2)^3^
   (c) (–3)^2^ × (–5)^2^

**Using laws of exponents, simplify and write the answer in exponential form:**

8. (a) 2^5^ × 2^3^
   (b) p^3^ × p^2^
   (c) 4^3^ × 4^2^
   (d) a^3^ × a^2^ × a^7^
   (e) 5^3^ × 5^7^ × 5^12^
   (f) (–4)^10^ × (–4)^20^
9. (a) 2^9^ ÷ 2^3^
   (b) 10^8^ ÷ 10^4^
   (c) 9^11^ ÷ 9^7^
   (d) 20^15^ ÷ 20^13^
   (e) 7^13^ ÷ 7^10^
   (f) 11^6^ ÷ 11^2^
10. (a) (6^2^)^4^
    (b) (2^2^)^100^
    (c) (7^50^)^2^
    (d) (5^3^)^7^
11. (a) 4^3^ × 2^3^
    (b) 2^5^ × b^5^
    (c) a^2^ × t^2^
    (d) 5^6^ × (–2)^6^
    (e) (–2)^4^ × (–3)^4^
    (f) a^m^ × b^m^
12. (a) 4^5^ ÷ 3^5^
    (b) 2^5^ ÷ b^5^
    (c) (–2)^5^ ÷ b^3^
    (d) 5^6^ ÷ (–2)^6^
13. (a) 8^0^
    (b) (−3)^0^
    (c) 4^0^ + 5^0^
    (d) 6^0 × 7^0^
14. (a) (4)^−1^
    (b) (−6)^−1^
    (c) $\Big(\frac{1}{3}\Big)^{-1}$
    (d) $\Big(\frac{-2}{3}\Big)^{-1}$
15. (a) 3^2^ × 3^4^ × 3^8^
    (b) 6^15^ ÷ 6^10^
    (c) a^3^ × a^2^
    (d) 7^x^ × 7^2^
    (e) (5^2^)^3^ ÷ 5^3^
    (f) 2^5^ × 5^5^
    (g) a^4^ × b^4^
    (h) (3^4^)^3^
    (i) (2^20^ ÷ 2^15^) × 2^3^
    (k) 8^t^ ÷ 8^2^
16. Express each of the following as a product of prime factors only in exponential form:
    (a) 108 × 192
    (b) 270
    (c) 729 × 64
    (d) 768
17. Simplify:
    (a) $\frac{(2^5)^2 \times 7^3}{8^3 \times 7}$
    (b) $\frac{25 \times 5^2 \times t^8}{10^3 \times t^4}$
    (c) $\frac{3^5 \times 10^5 \times 25}{5^7 \times 6^5}$
18. Write the following numbers in the expanded forms:
    - 279404,
    - 3006194,
    - 2806196,
    - 120719,
    - 20068
19. Find the number from each of the following expanded forms:
    (a) 8 × 10^4^ + 6 × 10^3^ + 0 × 10^2^ + 4 × 10^1^ + 5 × 10^0^
    (b) 4 × 10^5^ + 5 × 10^3^ + 3 × 10^2^ + 2 × 10^0^
    (c) 3 × 10^4^ + 7 × 10^2^ + 5 × 10^0^
    (d) 9 × 10^5^ + 2 × 10^2^ + 3 × 10^1^
20. Express the following numbers in standard form:
    (a) 5,00,00,000
    (b) 70,00,000
    (c) 3,18,65,00,000
    (d) 3,90,878
    (e) 39087.8
    (f) 3908.78
21. Expregs each of the following numbers in standard form:
    (a) Diameter of Earth = 12756000 m.
    (b) Distance between Earth and Moon = 384000000 m.
    (c) Population of India in March 2001 = 1027000000.
    (d) Number of stars in a galaxy = 100000000000.
    (e) The present age of universe = 12000000000 years.
