> Solve the following equation and verify your answer:

1. $\frac{2x + 5}{3} = 3x - 10$
2. $\frac{a - 8}{3} = \frac{a - 3}{2}$
3. $\frac{7y + 2}{5} = \frac{6y - 5}{11}$
4. $x - 2x + 2 - \frac{16}{3}x + 5 = 3 - \frac{7}{2}x$
5. $\frac{1}{2}x + 7x - 6 = 7x + \frac{1}{4}$
6. $\frac{3}{4}x + 4x = \frac{7}{8} + 6x - 6$
7. $\frac{7}{2}x - \frac{5}{2}x = \frac{20}{3}x + 10$
8. $\frac{6x + 1}{2} + 1 = \frac{7x - 3}{3}$
9. $\frac{3a - 2}{3} + \frac{2a + 3}{2} = a + \frac{7}{6}$
10. $x - \frac{(x - 1)}{2} = 1 - \frac{(x - 2)}{3}$
11. $\frac{3x}{4} - \frac{(x - 1)}{2} = \frac{(x - 2)}{3}$
12. $\frac{5x}{3} - \frac{(x - 1)}{4} = \frac{(x - 3)}{5}$
13. $\frac{(3x + 1)}{16} + \frac{(2x - 3)}{7} = \frac{(x + 3)}{8} + \frac{(3x - 1)}{14}$
14. $\frac{(1 - 2x)}{7} - \frac{(2 - 3x)}{8} = \frac{3}{2} + \frac{x}{4}$
15. $\frac{9x + 7}{2} - \Big(x - \frac{x - 2}{7}\Big) = 36$
16. $0.18(5x - 4) = 0.5x + 0.8$
17. $\frac{2}{3x} - \frac{3}{2x} = \frac{1}{12}$
18. $\frac{4x}{9} + \frac{1}{3} + \frac{13}{108}x = \frac{8x + 19}{18}$
19. $\frac{(45 - 2x)}{15} - \frac{(4x + 10)}{5} = \frac{(15 - 14x)}{9}$
20. $5\Big(\frac{7x + 5}{3}\Big) - \frac{23}{3} = 13 - \frac{4x - 2}{3}$
21. $\frac{7x - 1}{4} - \frac{1}{3}\Big(2x - \frac{1 - x}{2}\Big) = \frac{10}{3}$
22. $\frac{0.5(x - 0.4)}{0.35} - \frac{0.6(x - 2.71)}{0.42} = x + 6.1$
23. $0.6x + \frac{19.5x - 32.5}{2} = 6.5x + 13 + \Big(\frac{13x - 26}{2}\Big)$
24. $(3x - 8)(3x - 2) - (4x - 11)(2x + 1) = (x - 3)(x + 7)$
25. $[(2x + 3) + (x + 5)]^2 + [(2x + 3) - (x + 5)]^2 = 10x^2 + 92$

> Solve the following equation and verify your answer:

1. $\frac{2x - 3}{3x + 2}$ = −$\frac{2}{3}$
2. $\frac{2 - y}{y + 7}$ = $\frac{3}{5}$
3. $\frac{5x - 7}{3x}$ = 2
4. $\frac{3x + 5}{2x + 7}$ = 4
5. $\frac{2y + 5}{y + 4}$ = 1
6. $\frac{2x + 1}{3x - 2}$ = $\frac{5}{9}$
7. $\frac{1 - 9y}{19 - 3y}$ = $\frac{5}{8}$
8. $\frac{2x}{3x + 1}$ = −3
9. $\frac{y - (7 - 8y)}{9y - (3 + 4y)}$ = $\frac{2}{3}$
10. $\frac{6}{2x - (3 - 4x)}$ = $\frac{2}{3}$
11. $\frac{2}{3x} - \frac{3}{2x}$ = $\frac{1}{12}$
12. $\frac{3x + 5}{4x + 2}$ = $\frac{3x + 4}{4x + 7}$
13. $\frac{7x - 2}{5x - 1}$ = $\frac{7x + 3}{5x + 4}$
14. $\Big(\frac{x + 1}{x + 2}\Big)^2$ = $\frac{x + 2}{x + 4}$
15. $\Big(\frac{x + 1}{x - 4}\Big)^2$ = $\frac{x + 8}{x - 2}$
16. $\frac{9x - 7}{3x + 5}$ = $\frac{3x - 4}{x + 6}$
17. $\frac{x + 2}{x + 5}$ = $\frac{x}{x + 6}$
18. $\frac{2x - (7 - 5x)}{9x - (3 + 4x)}$ = $\frac{7}{6}$
19. $\frac{15(2 - x) - 5(x + 6)}{1 - 3x}$ = 10
20. $\frac{x + 3}{x - 3} + \frac{x + 2}{x - 2}$ = 2
21. $\frac{(x + 2)(2x - 3) - 2x^2 + 6}{x - 5}$ = 2
22. $\frac{x^2 - (x + 1)(x + 2)}{5x + 1}$ = 6
23. $\frac{(2x + 3) - (5x - 7)}{6x + 11}$ = −$\frac{8}{3}$
24. Find a positive value of x for which the given equation is satisfied:
    1. $\frac{x^2 - 9}{5 + x^2}$ = −$\frac{5}{9}$
    2. $\frac{y^2 + 4}{3y^2 + 7}$ = $\frac{1}{2}$
