> Solve each of the following equations and check your answers:

1. x − 3 = 5
2. x − $\frac{3}{5}$ = $\frac{7}{5}$
3. 3x = 0
4. $\frac{x}{2}$ = 0
5. x − $\frac{1}{3}$ = $\frac{2}{3}$
6. x + $\frac{1}{2}$ = $\frac{7}{2}$
7. 10 − y = 6
8. 10 − y = 6
9. 7 + 4y = −5
10. $\frac{4}{5}$ − x = $\frac{3}{5}$
11. 2y − $\frac{1}{2}$ = −$\frac{1}{3}$
12. 14 = $\frac{7x}{10}$ − 8
13. 3(x + 2) = 15
14. $\frac{x}{4}$ = $\frac{7}{8}$
15. $\frac{1}{3}$ − 2x = 0
16. 3(x + 6) = 24
17. 3(x + 2) − 2(x − 1) = 7
18. 8(2x − 5) − 6(3x − 7) = 1
19. 6(1 − 4x) + 7(2 + 5x) = 53
20. 5(2 − 3x) − 17(2x − 5) = 16
21. $\frac{x − 3}{5}$ − 2 = −1
22. 5(x − 2) + 3(x + 1) = 25

> Solve the following equation and verify your answer:

1. 6x + 5 = 2x + 17
2. 2(5x − 3) − 3(2x − 1) = 9
3. $\frac{x}{2}$ = $\frac{x}{3}$ + 1
4. $\frac{x}{2}$ + $\frac{3}{2}$ = $\frac{2x}{5}$ − 1
5. $\frac{3}{4}$(x − 1) = x − 3
6. 3(x − 3) = 5(2x + 1)
7. 3x − 2(2x − 5) = 2(x + 3) − 8
8. x − $\frac{x}{4}$ − $\frac{1}{2}$ = 3 + $\frac{x}{4}$
9. $\frac{6x − 2}{9}$ + $\frac{3x + 5}{18}$ = $\frac{1}{3}$
10. m − $\frac{m − 1}{2}$ = 1 − $\frac{m − 2}{3}$
11. $\frac{(5x − 1)}{3}$ − $\frac{(2x − 3)}{3}$ = 1
12. 0.6x + $\frac{4}{5}$ = 0.28x + 1.16
13. 0.5x + $\frac{x}{3}$ = 0.25x + 7

# Exercise 7.20

Simplify each of the following algebraic expressions by removing grouping symbols.

1. 2x + (5x − 3y)
2. 3x − (y − 2x)
3. 5a − (3b − 2a + 4c)
4. −2 (x^2 − y^2 + xy) − 3(x^2 + y^2 − xy)
5. 3x + 2y − {x − (2y − 3)}
6. 5a − {3a − (2 − a) + 4}
7. a − [b − {a − (b − 1) + 3a}]
8. a − [2b − {3a − (2b − 3c)}]
9. −x + [5y − {2x − (3y − 5x)}]
10. 2a − [4b − {4a − 3(2a − b)}]
11. −a − [a + {a + b − 2a − (a − 2b)} − b]
12. 2x − 3y − [3x − 2y − {x − z − (x − 2y)}]
13. 5 + [x − {2y − (6x + y − 4) + 2x} − {x − (y − 2)}]
14. x^2 − [3x + {2x − (x^2 − 1) + 2}]
15. 20 − [5xy + 3{x^2 − (xy − y) − (x − y)}]
16. 85 − [12x − 7(8x − 3) − 2 {10x − 5(2 − 4x)}]
17. xy [yz − zx − {yx − (3y − xz) − (xy − zy)}]
